template-coq/theories/Ast.v
@@ -170,7 +170,14 @@ Record mutual_inductive_entry := {
 Module TemplateTerm <: Term.
 
   Definition term := term.
+
+  Definition tRel := tRel.
   Definition tSort := tSort.
+  Definition tProd := tProd.
+  Definition tLetIn := tLetIn.
+  Definition tInd := tInd.
+
+  Definition mkApps := mkApps.
 
 End TemplateTerm.
 
